got transfer function up with 2 admits

experimental/examples/token/Token.fst
@@ -36,17 +36,15 @@ type address = string
 
 type accounts = Map.ordmap address nat string_cmp
 
-// val add_account_values : Map.ordmap address int string_cmp -> int
-// let add_account_values accounts = MapProp.fold (fun _k v acc -> v + acc) accounts 0
-
 // we have to specify they are nats :(
 val add_account_values : Map.ordmap address nat string_cmp -> nat
 let add_account_values accounts =
  MapProp.fold (fun _key (v : nat) (acc : nat) -> v + acc) accounts 0
 
+
 unopteq type storage = {
   total_supply : nat;
-  accounts     : a : Map.ordmap address nat string_cmp { total_supply = add_account_values a }
+  accounts : a : accounts { total_supply = add_account_values a };
 }
 
 val emtpy_storage : storage
@@ -54,3 +52,106 @@ let empty_storage = {
   total_supply = 0;
   accounts = Map.empty;
 }
+
+unopteq type token = {
+  storage : storage;
+  version : nat;  // version of the token contract
+  name    : string;
+  symbol  : Char.char;
+}
+
+
+val has_n : accounts -> address -> nat -> bool
+let has_n accounts add to_transfer =
+  match Map.select add accounts with
+  | Some n -> to_transfer <= n
+  | None   -> false
+
+// useless lemma, thought i needed it, but I just did to_transfer >= n.
+// in the function above by accident.
+val has_more : sto : storage
+             -> add : address
+             -> num : nat
+             -> Lemma
+               (requires (has_n sto.accounts add num))
+               (ensures  (num <= Some?.v (Map.select add sto.accounts)))
+let has_more sto add num = ()
+
+
+val account_sub : acc : accounts
+                -> add : address
+                -> num : nat {has_n acc add num}
+                -> accounts
+let account_sub accounts add number =
+  match Map.select add accounts with
+  | Some balance -> Map.update add (balance - number) accounts
+
+
+val transfer_sub : acc : accounts
+                 -> add : address
+                 -> num : nat
+                 -> Lemma
+                  (requires (has_n acc add num))
+                  (ensures ( (add_account_values acc - num)
+                           == add_account_values (account_sub acc add num)))
+let transfer_sub acc add num =
+  match Map.select add acc with
+  | Some balance ->
+    let remaining : nat = balance - num in
+    admit ()
+
+
+val account_add : acc : accounts
+                -> add : address
+                -> num : nat
+                -> accounts
+let account_add acc add num =
+  match Map.select add acc with
+  | Some b' -> Map.update add (b' + num) acc
+  | None    -> Map.update add num        acc
+
+val transfer_add : acc : accounts
+                 -> add : address
+                 -> num : nat
+                 -> Lemma
+                  (ensures ( (add_account_values acc + num)
+                           == add_account_values (account_add acc add num)))
+
+let transfer_add acc add num =
+  match Map.select add acc with
+  | Some balance -> admit ()
+  | None         -> admit ()
+
+
+val transfer_acc : acc     : accounts
+                -> add_from : address
+                -> add_to   : address
+                -> num      : nat {has_n acc add_from num}
+                -> accounts
+let transfer_acc accounts add_from add_to number =
+  let new_accounts = account_sub accounts add_from number in
+  account_add new_accounts add_to number
+
+val transfer_maintains_supply
+  : acc      : accounts
+  -> add_from : address
+  -> add_to   : address
+  -> num      : nat
+  -> Lemma
+    (requires (has_n acc add_from num))
+    (ensures (add_account_values acc == add_account_values (transfer_acc acc add_from add_to num)))
+let transfer_maintains_supply acc add_from add_to num =
+  transfer_sub acc add_from num;
+  transfer_add (account_sub acc add_from num) add_to num
+
+val transfer
+  : stor     : storage
+  -> add_from : address
+  -> add_to   : address
+  -> num      : nat {has_n stor.accounts add_from num}
+  -> storage
+let transfer stor add_from add_to num =
+  let new_acc = account_add (account_sub stor.accounts add_from num) add_to num in
+  transfer_maintains_supply stor.accounts add_from add_to num;
+  { total_supply = stor.total_supply;
+    accounts     = new_acc }
